clean up ch07 to use sets; exercisify

chapter07-async-clients/solutions/exercise01_solution.dfy
@@ -1,16 +1,20 @@
 //#title KV Spec with Asynchronous Client Interface
 //#desc Modify the KV spec to encode asynchronous client requests.
 
+// You are given datatypes to represent outstanding requests and completed
+// replies waiting to be delivered to the client. Your task is to fill out the
+// action predicates to model the asynchronous arrival of requests,
+// serialization (moment of processing) points, and delivery of replies.
+
 // Note that we're unconcerned with the protocol at the moment;
 // the goal here is only to modify the spec to capture linearizability,
 // a property that arises because client requests take time to process.
 
-//#start-elide TODO(manos) need to exercisify this experiment
 include "../../library/Library.dfy"
 
 // See chapter06-refine/exercises/exercise01 for documentation on this module.
-// Here I give concrete types because I want to play around with an instance
-// of this module.
+// (Here we give concrete types because we want to instantiatie the module for
+// pseudoliveness tests at the end.)
 module Types {
   type Key = string
 
@@ -27,6 +31,19 @@ module Types {
   {
     map key | key in AllKeys() :: DefaultValue()
   }
+
+  // The Input and Output types describe the application-visible interface to the service.
+  // The application chooses a nonce (so it can identify which replies belong to it --
+  // think something like an RPC ID), and fills in the input parameters. The output reply
+  // has a copy of the input (so the app can check the nonce) and any output result
+  // (e.g. the value of a query).
+  datatype Input =
+    | InsertRequest(nonce:int, key:Key, value:Value)
+    | QueryRequest(nonce:int, key:Key)
+
+  datatype Output =
+    | InsertReply(request: Input)
+    | QueryReply(request: Input, output: Value)
 }
 
 // This module defines a Map state machine that serves as the system specification.
@@ -39,67 +56,78 @@ module Types {
 module MapSpec {
   import opened Types
 
-// TODO(jonh)add nonce
-  datatype Input =
-    | InsertRequest(key:Key, value:Value)
-    | QueryRequest(key:Key)
-
-  datatype Output =
-    | InsertReply(request: Input)
-    | QueryReply(request: Input, output: Value)
-
   datatype Variables = Variables(mapp:map<Key, Value>,
-    requests:multiset<Input>, replies:multiset<Output>)
+    requests:set<Input>, replies:set<Output>)
     //TODO(jonh) go to set; prevent duplicate insertion
 
   predicate Init(v: Variables)
   {
     && v.mapp == InitialMap()
-    && v.requests == multiset{}
-    && v.replies == multiset{}
+//#exercise    // TODO Add stuff here
+//#start-elide
+    && v.requests == {}
+    && v.replies == {}
+//#end-elide
   }
 
   predicate AcceptRequest(v:Variables, v':Variables, request: Input)
   {
-    && v' == v.(requests := v.requests + multiset{request})
+//#exercise    false // TODO Define this predicate
+//#start-elide
+    && request !in v.requests // (liveness only) if client picked identical nonces, don't let the requests collapse.
+    && v' == v.(requests := v.requests + {request})
+//#end-elide
   }
 
   predicate DeliverReply(v:Variables, v':Variables, reply: Output)
   {
+//#exercise    false // TODO Define this predicate
+//#start-elide
     && reply in v.replies
-    && v' == v.(replies := v.replies - multiset{reply})
+    && v' == v.(replies := v.replies - {reply})
+//#end-elide
   }
 
   predicate InsertOp(v:Variables, v':Variables, request: Input)
   {
+//#exercise    false // TODO Replace me. Reference chapter06/exercises/exercise01.dfy InsertOp.
+//#start-elide
     // A well-formed condition: we're not even gonna talk about keys other than AllKeys().
     && request.key in AllKeys()
     // Don't do a request that a client hasn't asked for.
     && request in v.requests
     && request.InsertRequest?
+    && var reply := InsertReply(request);
+    && reply !in v.replies  // (liveness only) if client picked identical nonces, don't let a reply "catch up" with another and collapse.
     && v' == v.(
       // Replace key with value. v.mapp domain remains AllKeys().
       mapp := v.mapp[request.key := request.value],
       // Remove request from those awaiting service
-      requests := v.requests - multiset{request},
+      requests := v.requests - {request},
       // Add reply marking Insert complete so client can learn about it
-      replies := v.replies + multiset{InsertReply(request)})
+      replies := v.replies + {reply})
+//#end-elide
   }
 
   predicate QueryOp(v:Variables, v':Variables, request: Input, output: Value)
   {
+//#exercise    false // TODO Replace me. Reference chapter06/exercises/exercise01.dfy QueryOp.
+//#start-elide
     && request.key in AllKeys()
     && request.key in v.mapp
     // Don't do a request that a client hasn't asked for.
     && request in v.requests
     && request.QueryRequest?
+    && var reply := QueryReply(request, output);
+    && reply !in v.replies  // (liveness only) if client picked identical nonces, don't let a reply "catch up" with another and collapse.
     && output == v.mapp[request.key]
     && v' == v.(
       // (No change to mapp state)
       // Remove request from those awaiting service
-      requests := v.requests - multiset{request},
+      requests := v.requests - {request},
       // Add reply marking Insert complete so client can learn about it
-      replies := v.replies + multiset{QueryReply(request, output)})
+      replies := v.replies + {reply})
+//#end-elide
   }
 
   datatype Step =
@@ -124,8 +152,13 @@ module MapSpec {
     exists step :: NextStep(v, v', step)
   }
 
-  // We'll realize behaviors explicitly (as a sequence of states) so we can goof around
-  // with proofs about what this spec might say.
+  // Here are some point tests to confirm that the protocol allows various
+  // desired behavior: two possible resulting states for runs with overlapping
+  // insert requests, and one possible state for a run with non-overlapping
+  // insert requests.
+
+  // We'll materialize behaviors explicitly (as a sequence of states) so we can
+  // goof around with proofs about what this spec might say.
   predicate ValidBehavior(execution:seq<Variables>, steps:seq<Step>)
   {
     && |execution| == |steps| + 1
@@ -133,20 +166,19 @@ module MapSpec {
     && (forall i | 0<=i<|steps| :: NextStep(execution[i], execution[i+1], steps[i]))
   }
 
-  // Some point tests to confirm that the protocol allows various desired behavior.
   lemma PseudoLiveness()
   {
     // Here's a run that orders a simultaneously-outstanding set of inserts one way.
-    var req3 := InsertRequest("cat", 3);
-    var req4 := InsertRequest("cat", 4);
+    var req3 := InsertRequest(100, "cat", 3);
+    var req4 := InsertRequest(101, "cat", 4);
     var executionA := [
-      Variables(InitialMap(), multiset{}, multiset{}),
-      Variables(InitialMap(), multiset{req4}, multiset{}),
-      Variables(InitialMap(), multiset{req3, req4}, multiset{}),
-      Variables(InitialMap()["cat" := 4], multiset{req3}, multiset{InsertReply(req4)}),
-      Variables(InitialMap()["cat" := 3], multiset{}, multiset{InsertReply(req4), InsertReply(req3)}),
-      Variables(InitialMap()["cat" := 3], multiset{}, multiset{InsertReply(req3)}),
-      Variables(InitialMap()["cat" := 3], multiset{}, multiset{})
+      Variables(InitialMap(), {}, {}),
+      Variables(InitialMap(), {req4}, {}),
+      Variables(InitialMap(), {req3, req4}, {}),
+      Variables(InitialMap()["cat" := 4], {req3}, {InsertReply(req4)}),
+      Variables(InitialMap()["cat" := 3], {}, {InsertReply(req4), InsertReply(req3)}),
+      Variables(InitialMap()["cat" := 3], {}, {InsertReply(req3)}),
+      Variables(InitialMap()["cat" := 3], {}, {})
       ];
     var stepsA := [
       AcceptRequestStep(req4),
@@ -162,13 +194,13 @@ module MapSpec {
     // different value for cat at the end. I could also actually *query* the
     // cat, but I'm too lazy.
     var executionB := [
-      Variables(InitialMap(), multiset{}, multiset{}),
-      Variables(InitialMap(), multiset{req4}, multiset{}),
-      Variables(InitialMap(), multiset{req3, req4}, multiset{}),
-      Variables(InitialMap()["cat" := 3], multiset{req4}, multiset{InsertReply(req3)}),
-      Variables(InitialMap()["cat" := 4], multiset{}, multiset{InsertReply(req4), InsertReply(req3)}),
-      Variables(InitialMap()["cat" := 4], multiset{}, multiset{InsertReply(req3)}),
-      Variables(InitialMap()["cat" := 4], multiset{}, multiset{})
+      Variables(InitialMap(), {}, {}),
+      Variables(InitialMap(), {req4}, {}),
+      Variables(InitialMap(), {req3, req4}, {}),
+      Variables(InitialMap()["cat" := 3], {req4}, {InsertReply(req3)}),
+      Variables(InitialMap()["cat" := 4], {}, {InsertReply(req4), InsertReply(req3)}),
+      Variables(InitialMap()["cat" := 4], {}, {InsertReply(req3)}),
+      Variables(InitialMap()["cat" := 4], {}, {})
       ];
     var stepsB := [
       AcceptRequestStep(req4),
@@ -182,13 +214,13 @@ module MapSpec {
 
   // Here one request completes before the other; only one outcome is possible.
     var executionC := [
-      Variables(InitialMap(), multiset{}, multiset{}),
-      Variables(InitialMap(), multiset{req3}, multiset{}),
-      Variables(InitialMap()["cat" := 3], multiset{}, multiset{InsertReply(req3)}),
-      Variables(InitialMap()["cat" := 3], multiset{}, multiset{}),
-      Variables(InitialMap()["cat" := 3], multiset{req4}, multiset{}),
-      Variables(InitialMap()["cat" := 4], multiset{}, multiset{InsertReply(req4)}),
-      Variables(InitialMap()["cat" := 4], multiset{}, multiset{})
+      Variables(InitialMap(), {}, {}),
+      Variables(InitialMap(), {req3}, {}),
+      Variables(InitialMap()["cat" := 3], {}, {InsertReply(req3)}),
+      Variables(InitialMap()["cat" := 3], {}, {}),
+      Variables(InitialMap()["cat" := 3], {req4}, {}),
+      Variables(InitialMap()["cat" := 4], {}, {InsertReply(req4)}),
+      Variables(InitialMap()["cat" := 4], {}, {})
       ];
     var stepsC := [
       AcceptRequestStep(req3),
@@ -201,4 +233,3 @@ module MapSpec {
     assert ValidBehavior(executionC, stepsC);
   }
 }
-//#end-elide TODO(manos) need to exercisify this experiment
